updating import structure to improve tactic performance, consolidating in more proofs

src/computational_monads/simulation_semantics/is_tracking.lean
@@ -3,26 +3,33 @@ Copyright (c) 2023 Devon Tuma. All rights reserved.
 Released under Apache 2.0 license as described in the file LICENSE.
 Authors: Devon Tuma
 -/
-import computational_monads.simulation_semantics.simulate.induction.support
-import computational_monads.simulation_semantics.simulate.induction.eval_dist
+import computational_monads.simulation_semantics.simulate.induction
 import computational_monads.simulation_semantics.simulate.subsingleton
 
 /-!
 # Tracking Simulation Oracles
 
 This file defines a typeclass `sim_oracle.is_tracking` for oracles in which the
-query responses are independent of the current oracle state. For example in `loggingₛₒ`
-the internal state doesn't change the input and output, it just records them.
+query responses are independent of the current oracle state.
+This is represented by giving functions `query_f` and `state_f` that correspond to these pieces,
+and a statement `apply_dist_equiv_state_f_map_query_f` that shows that the oracle function
+actually splits into the two components given.
+
+For example in `loggingₛₒ` the internal state doesn't change the main output, it just records it.
 This allows for many lemmas to be automatically shared between these sorts of oracles.
 `sim_oracle.is_stateless` extends this further to oracles with no internal state at all.
--/
 
-variables {α β γ : Type} {spec spec' spec'' : oracle_spec} {S S' : Type}
+We also construct a `tracking_oracle` that creates a simulation oracle from a direct specification
+of `query_f` and `state_f`, that satisfies `is_tracking` by construction.
+This is convenient in defining e.g. `loggingₛₒ` and `idₛₒ`
+-/
 
 open_locale big_operators ennreal
 open oracle_comp oracle_spec
 
 namespace sim_oracle
+
+variables {α β γ : Type} {spec spec' spec'' : oracle_spec} {S S' : Type}
 
 /-- Typeclass for oracles in which the query responses are independent of the current oracle state.
 We define this in terms of the existence of two functions `query_f` and `state_f`
@@ -141,3 +148,176 @@ end simulate'
 end is_tracking
 
 end sim_oracle
+
+/-- Oracle where the query result is indepenent of the current oracle state,
+although the new state may depend upon the previous state.
+For example a logging oracle that just tracks the input and output of queries.
+`o` is the way the oracle responds to queries, which doesn't have access to the state.
+`update_state` takes a query and internal state and returns the new internal state.
+Note that `update_state` is not a probabalistic function, and has no oracle access -/
+def tracking_oracle {spec spec' : oracle_spec} {S : Type}
+  (o : Π (i : spec.ι), spec.domain i → oracle_comp spec' (spec.range i))
+  (update_state : Π (s : S) (i : spec.ι), spec.domain i → spec.range i → S)
+  (default_state : S) : sim_oracle spec spec' S :=
+{ default_state := default_state,
+  o := λ i ⟨t, s⟩, (λ u, (u, update_state s i t u)) <$> (o i t) }
+
+notation `⟪` o `|` update_state `,` default_state `⟫` :=
+  tracking_oracle o update_state default_state
+
+namespace tracking_oracle
+
+open_locale big_operators ennreal
+open oracle_comp oracle_spec
+
+variables {α β γ : Type} {spec spec' spec'' : oracle_spec}
+variables {S S' : Type} (o : Π (i : spec.ι), spec.domain i → oracle_comp spec' (spec.range i))
+  (o' : Π (i : spec.ι), spec.domain i → oracle_comp spec'' (spec.range i))
+  (update_state : Π (s : S) (i : spec.ι), spec.domain i → spec.range i → S)
+  (update_state' : Π (s : S') (i : spec.ι), spec.domain i → spec.range i → S')
+  (default_state : S) (default_state' : S') (a : α) (i : spec.ι) (t : spec.domain i)
+  (oa : oracle_comp spec α) (ob : α → oracle_comp spec β) (s : S) (s' : S')
+  (x : spec.domain i × S) (y : spec.range i × S)
+
+@[simp] lemma apply_eq : ⟪o | update_state, default_state⟫ i x =
+  (λ u, (u, update_state x.2 i x.1 u)) <$> (o i x.1) := by {cases x, refl}
+
+section support
+
+@[simp] lemma support_apply : (⟪o | update_state, default_state⟫ i x).support =
+  (λ u, (u, update_state x.2 i x.1 u)) '' (o i x.1).support :=
+set.ext (λ y, by rw [apply_eq, support_map])
+
+lemma fin_support_apply [decidable_eq S] :
+  (⟪o | update_state, default_state⟫ i x).fin_support =
+    (o i x.1).fin_support.image (λ u, (u, update_state x.2 i x.1 u)) :=
+by simp only [fin_support_eq_iff_support_eq_coe, apply_eq, support_map,
+  finset.coe_image, coe_fin_support_eq_support]
+
+lemma mem_support_apply_iff {y : spec.range i × S} :
+  y ∈ (⟪o | update_state, default_state⟫ i x).support ↔
+    y.1 ∈ (o i x.1).support ∧ update_state x.2 i x.1 y.1 = y.2 :=
+by simp only [support_apply, prod.eq_iff_fst_eq_snd_eq, set.mem_image,
+  and_comm (_ = y.fst), exists_eq_right_right]
+
+/-- If the oracle can take on any value then the first element of the support is unchanged -/
+lemma support_simulate'_eq_support (h : ∀ i t, (o i t).support = ⊤) :
+  (simulate' ⟪o | update_state, default_state⟫ oa s).support = oa.support :=
+sorry
+-- support_simulate'_eq_support _ oa s (λ i t s, set.ext (λ x, by simp only
+--   [h, set.top_eq_univ, set.mem_univ, true_and, apply_eq, support_map, set.mem_image,
+--     prod.exists, prod.mk.inj_iff, exists_eq_left, exists_eq_left', exists_apply_eq_apply]))
+
+/-- Particular case of `support_simulate'_eq_support` for `query`.
+In particular a tracking oracle that *only* does tracking doesn't affect the main output. -/
+@[simp] lemma support_simulate'_query_eq_support :
+  (simulate' ⟪query | update_state, default_state⟫ oa s).support = oa.support :=
+support_simulate'_eq_support query update_state default_state oa s (λ _ _, rfl)
+
+lemma support_simulate'_eq_support_simulate' (h : ∀ i t, (o i t).support = (o' i t).support) :
+  (simulate' ⟪o | update_state, default_state⟫ oa s).support =
+    (simulate' ⟪o' | update_state', default_state'⟫ oa s').support :=
+support_simulate'_eq_support_simulate' (λ i t s s', set.ext $ λ x,
+  by simp only [mem_support_apply_iff, h, simulate'_query, support_map, support_apply,
+    set.mem_image, set.mem_set_of_eq, prod.exists, exists_and_distrib_right, exists_eq_right,
+    exists_eq_right', exists_eq_right_right, prod.eq_iff_fst_eq_snd_eq, and_comm (_ = x)]) oa s s'
+
+/-- The support of `simulate'` is independt of the tracking functions -/
+lemma support_simulate'_eq_support_simulate'_of_oracle_eq :
+  (simulate' ⟪o | update_state, default_state⟫ oa s).support =
+    (simulate' ⟪o | update_state', default_state'⟫ oa s').support :=
+support_simulate'_eq_support_simulate' o o _ _ _ _ oa s s' (λ _ _, rfl)
+
+section subsingleton
+
+variables [subsingleton S]
+
+@[simp] lemma support_apply_of_subsingleton :
+  (⟪o | update_state, default_state⟫ i x).support = prod.fst ⁻¹' (o i x.1).support :=
+set.ext (λ y, by erw [apply_eq, map_eq_bind_return_comp,
+  support_bind_prod_mk_of_snd_subsingleton, set.image_id])
+
+lemma support_simulate_eq_preimage_support_of_subsingleton (h : ∀ i t, (o i t).support = ⊤) :
+  (simulate ⟪o | update_state, default_state⟫ oa s).support = prod.fst ⁻¹' oa.support :=
+by rw [set.preimage, support_simulate_eq_support_simulate'_of_subsingleton,
+  support_simulate'_eq_support o _ _ oa s h]
+
+@[simp] lemma support_simulate_query_eq_support_of_subsingleton :
+  (simulate ⟪query | update_state, default_state⟫ oa s).support = prod.fst ⁻¹' oa.support :=
+support_simulate_eq_preimage_support_of_subsingleton query _ _ oa s (λ _ _, rfl)
+
+end subsingleton
+
+end support
+
+section eval_dist
+
+@[simp] lemma eval_dist_apply :
+  ⁅⟪o | update_state, default_state⟫ i (t, s)⁆ = ⁅o i t⁆.map (λ u, (u, update_state s i t u)) :=
+by rw [apply_eq, eval_dist_map]
+
+/-- If the oracle has uniform distribution, then the distribution under `simulate'` is unchanged -/
+lemma eval_dist_simulate'_eq_eval_dist
+  (h : ∀ i t, ⁅o i t⁆ = pmf.uniform_of_fintype (spec.range i)) :
+  ⁅simulate' ⟪o | update_state, default_state⟫ oa s⁆ = ⁅oa⁆ :=
+sorry
+-- eval_dist_simulate'_eq_eval_dist _ oa s (λ i t s, trans
+--   (by simpa [eval_dist_apply, pmf.map_comp] using pmf.map_id ⁅o i t⁆) (h i t))
+
+/-- Specific case of `eval_dist_simulate'_eq_eval_dist` for query.
+In particular if a tracking oracle *only* does tracking gives the same main output distribution. -/
+@[simp] lemma eval_dist_simulate'_query_eq_eval_dist :
+  ⁅simulate' ⟪query | update_state, default_state⟫ oa s⁆ = ⁅oa⁆ :=
+eval_dist_simulate'_eq_eval_dist query update_state default_state oa s (λ _ _, rfl)
+
+lemma eval_dist_simulate'_eq_eval_dist_simulate'
+  (h : ∀ i t, o i t ≃ₚ o' i t) : simulate' ⟪o | update_state, default_state⟫ oa s ≃ₚ
+    simulate' ⟪o' | update_state', default_state'⟫ oa s' :=
+sorry
+-- -- eval_dist_simulate'_eq_eval_dist_simulate' (λ i t s s',
+--   by simp [pmf.map_comp, tracking_oracle.apply_eq, eval_dist_map, (h i t).eval_dist_eq]) _ _ _
+
+/-- The first output of simulation under different `tracking_oracle` with the same oracle
+is the same regardless of if the tracking functions are different. -/
+lemma eval_dist_simulate'_eq_eval_dist_simulate'_of_oracle_eq :
+  ⁅simulate' ⟪o | update_state, default_state⟫ oa s⁆ =
+    ⁅simulate' ⟪o | update_state', default_state'⟫ oa s'⁆ :=
+eval_dist_simulate'_eq_eval_dist_simulate' o o _ _ _ _ oa s s' (λ _ _, rfl)
+
+end eval_dist
+
+section prob_event
+
+variable (e : set α)
+
+@[simp] lemma prob_event_apply (e : set (spec.range i × S)) :
+  ⁅e | ⟪o | update_state, default_state⟫ i (t, s)⁆ =
+    ⁅λ u, (u, update_state s i t u) ∈ e | o i t⁆ :=
+by simpa only [apply_eq, prob_event_map]
+
+lemma prob_event_simulate'_eq_prob_event
+  (h : ∀ i t, ⁅o i t⁆ = pmf.uniform_of_fintype (spec.range i)) :
+  ⁅e | simulate' ⟪o | update_state, default_state⟫ oa s⁆ = ⁅e | oa⁆ :=
+prob_event_eq_of_eval_dist_eq (eval_dist_simulate'_eq_eval_dist _ _ _ _ _ h) e
+
+/-- Specific case of `eval_dist_simulate'_eq_eval_dist` for query.
+In particular if a tracking oracle *only* does tracking gives the same main output distribution. -/
+lemma prob_event_simulate'_query_eq_prob_event :
+  ⁅e | simulate' ⟪query | update_state, default_state⟫ oa s⁆ = ⁅e | oa⁆ :=
+prob_event_simulate'_eq_prob_event _ _ _ oa s e (λ _ _, rfl)
+
+lemma prob_event_simulate'_eq_prob_event_simulate'
+  (h : ∀ i t, o i t ≃ₚ o' i t) : ⁅e | simulate' ⟪o | update_state, default_state⟫ oa s⁆ =
+    ⁅e | simulate' ⟪o' | update_state', default_state'⟫ oa s'⁆ :=
+prob_event_eq_of_eval_dist_eq (eval_dist_simulate'_eq_eval_dist_simulate' _ _ _ _ _ _ _ _ _ h) e
+
+/-- The first output of simulation under different `tracking_oracle` with the same oracle
+is the same regardless of if the tracking functions are different. -/
+lemma prob_event_simulate'_eq_eval_dist_simulate'_of_oracle_eq :
+  ⁅e | simulate' ⟪o | update_state, default_state⟫ oa s⁆ =
+    ⁅e | simulate' ⟪o | update_state', default_state'⟫ oa s'⁆ :=
+prob_event_simulate'_eq_prob_event_simulate' o o _ _ _ _ oa s s' e (λ _ _, rfl)
+
+end prob_event
+
+end tracking_oracle
