src/computational_monads/simulation_semantics/constructions/logging/counting_oracle.lean
@@ -3,7 +3,7 @@ Copyright (c) 2022 Devon Tuma. All rights reserved.
 Released under Apache 2.0 license as described in the file LICENSE.
 Authors: Devon Tuma
 -/
-import computational_monads.simulation_semantics.constructions.tracking_oracle
+import computational_monads.simulation_semantics.is_tracking
 import computational_monads.query_tracking.query_count.order
 
 /-!
